finished the if rule, modulo a couple of assumptions that need to be added regarding starting in a valid state.

CPS_Ctl/ImpCtl.thy
@@ -35,6 +35,8 @@ datatype syn' =
   | Sskip
   | Swhile
 
+type_synonym 'x imp_state' = "'x gensyn list * bool"
+
 type_synonym 'x state' = "'x gensyn list * bool * int"
 
 (* TODO: finish while case *)
@@ -45,11 +47,11 @@ while ==
 - push while [body]
 - push while [cond, body]
 *)
-definition imp_ctl_sem :: "syn' \<Rightarrow> 'x state' \<Rightarrow> 'x state'" where
+definition imp_ctl_sem :: "syn' \<Rightarrow> 'x imp_state' \<Rightarrow> 'x imp_state'" where
 "imp_ctl_sem x st =
   (case st of
-    ([], b, i) \<Rightarrow> ([], b, i)
-    | ((G z l)#t, b, i) \<Rightarrow>
+    ([], b) \<Rightarrow> ([], b)
+    | ((G z l)#t, b) \<Rightarrow>
       ((case x of
         Sskip \<Rightarrow> t
         | Sif \<Rightarrow>
@@ -62,55 +64,21 @@ definition imp_ctl_sem :: "syn' \<Rightarrow> 'x state' \<Rightarrow> 'x state'"
          [body] \<Rightarrow> (if b then body # (G z l) # t else t)
          | [cond, body] \<Rightarrow> cond # (G z [body]) # t
          | _ \<Rightarrow> [] \<comment> \<open> error \<close>))
-      , b, i))"
-
-(*
-definition imp_ctl_sem :: "syn' \<Rightarrow> state' \<Rightarrow> state'" where
-"imp_ctl_sem x st =
-  (case st of ((sk, GRPath cp, d), b) \<Rightarrow>
-    (case x of
-      Sskip \<Rightarrow> st
-      | Sif \<Rightarrow> 
-        (case d of
-         Down \<Rightarrow> ((sk, GRPath (cp @ [0]), Down), b)
-         | Up xcp \<Rightarrow>
-                 (case get_suffix cp xcp of
-                    Some (xcph#xcpt) \<Rightarrow>
-                      (case xcph of
-                          0 \<Rightarrow> \<comment> \<open>condition\<close>
-                            (if b 
-                             then ((sk, GRPath (cp @ [1]), Down), b)
-                             else ((sk, GRPath (cp @ [2]), Down), b))
-                          | _ \<Rightarrow> \<comment> \<open> then/else \<close>
-                              (case gensyn_cp_parent sk cp of
-                                None \<Rightarrow> ((sk, GRDone, Up cp), b)
-                                | Some cp' \<Rightarrow> ((sk, GRPath cp', Up cp), b)))))
-        | Swhile \<Rightarrow>
-          (case d of
-           Down \<Rightarrow> ((sk, GRPath (cp @ [0]), Down), b)
-           | Up xcp \<Rightarrow>
-                 (case get_suffix cp xcp of
-                    Some (xcph#xcpt) \<Rightarrow>
-                      (case xcph of
-                          0 \<Rightarrow> \<comment> \<open>condition\<close>
-                            (if b 
-                             then ((sk, GRPath (cp @ [1]), Down), b)
-                             else (case gensyn_cp_parent sk cp of
-                                     None \<Rightarrow> ((sk, GRDone, Up cp), b)
-                                     | Some cp' \<Rightarrow> ((sk, GRPath cp', Up cp), b)))
-                          | _ \<Rightarrow> \<comment> \<open> loop body\<close>
-                              ((sk, GRPath cp, Down), b))))))"
-*)
+      , b))"
 
 datatype syn = 
   Simp syn'
   | Scond cond_syn'
   | Seq "Seq.syn"
 
-type_synonym 'x state = 
-  "('x, (bool md_triv option md_prio * int md_triv option md_prio)) control"
+type_synonym ('s, 'x) state = 
+  "('s, (bool md_triv option md_prio * int md_triv option md_prio * 'x)) control"
 
-definition imp_trans :: "syn \<Rightarrow> syn'" where
+type_synonym ('s) cstate = 
+  "('s, unit option) state"
+
+
+definition imp_trans :: "ImpCtl.syn \<Rightarrow> ImpCtl.syn'" where
 "imp_trans s =
   (case s of
     Simp s' \<Rightarrow> s'
@@ -127,84 +95,69 @@ definition seq_trans :: "syn \<Rightarrow> Seq.syn" where
   (case s of
     Seq x \<Rightarrow> x
     | _ \<Rightarrow> Seq.Sskip)"
-(*
-definition printcalcseq_sem_l :: "syn \<Rightarrow> state \<Rightarrow> state" where
-"printcalcseq_sem_l =
-  lift_map_s printcalc_trans
-     (prod_l id_l (snd_l id_l))
-     (pcomp print_calc_seq_lc)"
-*)
+
 definition imp_prio :: "(syn' \<Rightarrow> nat)" where
 "imp_prio x =
 (case x of
     Sskip \<Rightarrow> 0
     | _ \<Rightarrow> 2)"
 
-(*
-definition imp_sem_l :: "syn \<Rightarrow> 'x state \<Rightarrow> 'x state" where
-"imp_sem_l =
-  lift_map_s imp_trans
-    (schem_lift (SP (SP NA (SP NB NC)) ND)
-                (SP (SP (SO NA) (SP (SPRC imp_prio (SO NB)) (SPRC imp_prio (SO NC))))
-                  (SP (SPRK (SO ND)) NX)))
-    imp_ctl_sem"
-*)
+(* failed experiments in trying to coax the auto-lifter *)
 
+(*
 definition imp_sem_l :: "syn \<Rightarrow> 'x state \<Rightarrow> 'x state" where
 "imp_sem_l =
   lift_map_s imp_trans
     (schem_lift (SP NA (SP NB NC))
                 (SP (SPRC imp_prio (SO NA)) (SP (SPRK (SO NB)) (SPRK (SO NC)))))
   imp_ctl_sem"
+*)
+(*
+definition imp_sem_lifting_gen_huh ::  "(ImpCtl.syn', 'x gensyn list * int, 
+                                      ('a :: Pordb ) *
+                                      ('x gensyn list md_triv option md_prio * int md_triv option md_prio)) lifting" where
+"imp_sem_lifting_gen_huh = 
+ (schem_lift (SP NA NB) (SP NX (SP (SPRI (SO NA)) (SPRI (SO NB)))))"
+*)
 
 (*
-definition imp_sem_lifting_gen' :: "(syn, 'x state', ('x, 'y :: Pordb) control) lifting" where
-"imp_sem_lifting_gen' = schem_lift
-  (SP NA (SP NB NC)) (SP (SPRI (SO NA)) (SP (SPRK (SO NB)) (SPRK (SO (NC)))))"
+definition imp_sem_lifting_gen_huh ::  "(ImpCtl.syn', 'x gensyn list, 
+                                      ('x gensyn list md_triv option md_prio * 
+                                           ('a :: Pordb ))) lifting" where
+"imp_sem_lifting_gen_huh = 
+ (schem_lift NA (SP (SPRI (SO NA)) NX))"
 *)
-(* (a, b) control =
-  (a gensyn list md_triv option md_prio * b)
-*)
-
-(* TODO: it's not letting us name the "extra part at the end" parameter 'y.
-but a blank pattern is fine
-i don't understand why. 
-i'm going to roll with this for now.
-*)
-definition imp_sem_lifting_gen' :: "(syn', 'x state', 
-                                      ('x, bool md_triv option md_prio * 
-                                           int md_triv option md_prio * 
-                                           (_ :: Pordb)) control) lifting" where
-"imp_sem_lifting_gen' = 
- (schem_lift (SP NA (SP NB NC))
-                (SP (SPRC imp_prio (SO NA)) (SP (SPRK (SO NB)) (SP (SPRK (SO NC)) NX))))"
 
 
-term "[imp_sem_lifting_gen', seq_sem_lifting_gen']"
 
-definition seq_sem_l :: "syn \<Rightarrow> 'x state \<Rightarrow> 'x state" where
-"seq_sem_l =
-  lift_map_s seq_trans
-    (schem_lift NA (SP (SPRI (SO NA)) NX))
-  seq_sem'"
+definition imp_sem_lifting_gen :: "(ImpCtl.syn', 'x imp_state', 
+                                   ('x, _ ) state) lifting" where
+"imp_sem_lifting_gen = 
+ (schem_lift (SP NA NB)
+             (SP (SPRC imp_prio (SO NA)) (SP (SPRK (SO NB)) NX)))"
 
-definition seq_sem_l' :: "syn \<Rightarrow> 'x state \<Rightarrow> 'x state" where
+
+definition imp_sem_l_gen :: "('s \<Rightarrow> ImpCtl.syn') \<Rightarrow> 's \<Rightarrow> ('x, 'z :: Mergeableb) state \<Rightarrow> ('x, 'z) state" where
+"imp_sem_l_gen lfts =
+  lift_map_s lfts
+    imp_sem_lifting_gen
+  imp_ctl_sem"
+
+
+definition seq_sem_l' :: "syn \<Rightarrow> ('x, 'z :: Mergeableb) state \<Rightarrow> ('x, 'z) state" where
 "seq_sem_l' = seq_sem_l_gen seq_trans"
 
-definition sems :: "(syn \<Rightarrow> 'x state \<Rightarrow> 'x state) list" where
-"sems = [seq_sem_l', imp_sem_l]"
+definition sems :: "(syn \<Rightarrow> ('x, 'z :: Mergeableb) state \<Rightarrow> ('x, 'z :: Mergeableb) state) list" where
+"sems = [seq_sem_l_gen seq_trans, imp_sem_l_gen imp_trans]"
 
 definition sem_final :: "(syn, 'x, bool md_triv option md_prio * 
-                                           int md_triv option md_prio) sem" where
+                                           int md_triv option md_prio
+                                    * unit option) sem" where
 "sem_final = \<lparr> s_sem = (pcomps' sems) \<rparr>"
 
 definition prog where
 "prog = (G (Seq Sseq) [(G (Seq Sseq) []), 
                         (G (Simp Sif) [(G (Seq Sseq) []), (G (Seq Sseq) [])])])"
-
-value "sem_exec (sem_final) 4 (mdp 0 (Some (mdt [prog])), (mdp 0 (Some (mdt False))))"
-
-value "sem_exec (sem_final) 5 (mdp 0 (Some (mdt [prog])), (mdp 0 (Some (mdt False))))"
 
 
 (* next: generalized version of If, While rules*)
@@ -212,17 +165,309 @@ value "sem_exec (sem_final) 5 (mdp 0 (Some (mdt [prog])), (mdp 0 (Some (mdt Fals
 (* also, we probably need to have a way to say that
    boolean expressions can't affect control flow (also in terms of domination?)
 *)
+
+definition get_cond :: 
+"bool md_triv option md_prio * 
+  int md_triv option md_prio * 
+  (_ :: Pordb) \<Rightarrow> bool option" where
+"get_cond st = 
+  (case st of
+    (b, _, _) \<Rightarrow> 
+    (case b of
+      (mdp _ (Some (mdt b'))) \<Rightarrow> Some b'
+      | _ \<Rightarrow> None))"
+
+term "imp_sem_l_gen"
+term "seq_sem_l_gen"
+(*
+do we need to take into account "separation" between imp and cond?
+we probably need to model cond running for possibly multiple steps.
+*)
+(* can we eliminate P2? *)
+(* probably not, unless we require P2 to be an expression language.
+   besides this should be fine. *)
+(* we need to enforce that the initial state is valid.
+that is, that it falls into the valid set given by the imp lifting. *)
 lemma HImp_gen :
   assumes H0 : "gs = \<lparr> s_sem = pcomps' fs \<rparr>"
   (*assumes H1 : "seq_sem_l_gen lfts \<in> set fs" *)
-  assumes HF : "f = seq_sem_l_gen lfts"
+  assumes HF : "f = imp_sem_l_gen lfts"
   assumes Hpres : "sups_pres (set fs)"
   assumes Hnemp : "g \<in> set fs"
-  assumes Hdom : "(f \<downharpoonleft> (set fs) Sseq')"
-  assumes H2 : "lfts Sseq' = Sseq"
-  assumes H : "|gs| {- P1 -} cs {- P2 -}"
-  shows "|gs| {- P1 -} [G Sseq' cs] {- P2 -}"
-proof
+  assumes Hdom : "(f \<downharpoonleft> (set fs) Sif')"
+  assumes Hsyn : "lfts Sif' = Sif"
+  (* TODO: generalize *)
 
+  assumes Hcond : "|gs| {- P1 -} [cond] {- P2 -}"
+  assumes Htrue : "|gs| {- (\<lambda> st . P2 st \<and> get_cond st = Some True) -} [body]
+                        {- P3 -}"
+  assumes Hfalse : "|gs| {- (\<lambda> st . P2 st \<and> get_cond st = Some False) -} [] {-P3-}"
+  shows "|gs| {- P1 -} [G Sif' [cond, body]] {- P3 -}"
+proof
+  fix c'
+  assume Guard : "|gs| {P3} c'"
+
+
+(* need to think about how we are structuring states. *)
+(* where will the data of interest be *)
+  have Gtrue : "|gs| {\<lambda>st. P2 st \<and> get_cond st = Some True} [body] @ c'"
+    using HTE[OF Htrue Guard] by auto
+
+  have Gfalse : "|gs| {\<lambda>st. P2 st \<and> get_cond st = Some False} [] @ c'"
+    using HTE[OF Hfalse Guard] by auto
+
+  show "|gs| {P1} [G Sif' [cond, body]] @ c'"
+  proof
+    fix m :: "('a, 'b) state"
+
+    assume M : "P1 (snd m)"
+    assume CM : "s_cont m = [G Sif' [cond, body]] @ c'"
+
+    show "(safe gs m)"
+    proof(cases "(sem_step gs m)")
+      case None
+
+      then have False using CM H0
+        by(auto simp add: sem_step_def)
+
+      then show ?thesis by auto
+    next
+      case (Some m')
+
+      have F_eq : "sem_step \<lparr> s_sem = f \<rparr> m = Some m'"
+        using sym[OF dominant_pcomps'[OF Hpres Hnemp Hdom]] CM Some H0
+        by(simp add: sem_step_def)
+
+      have CM' : "s_cont m' = [cond] @ ([ G Sif' [body]] @ c')" 
+        using CM Hsyn F_eq unfolding HF
+        by(cases m; cases m'; auto simp add: s_cont_def sem_step_def imp_sem_l_gen_def imp_ctl_sem_def imp_sem_lifting_gen_def
+           schem_lift_defs 
+          merge_l_def fst_l_def snd_l_def prio_l_def triv_l_def option_l_def
+          split: md_prio.splits md_triv.splits option.splits)
+
+      (* this will need to be shown using valid-sets. *)
+      have M'_valid : "\<And> p . fst (snd m) \<noteq> mdp p None" sorry
+
+      have Sm' : "snd m = snd m'"
+        using CM Hsyn F_eq M'_valid unfolding HF
+        by(cases m; cases m'; auto simp add: s_cont_def sem_step_def imp_sem_l_gen_def imp_ctl_sem_def imp_sem_lifting_gen_def
+           schem_lift_defs 
+          merge_l_def fst_l_def snd_l_def prio_l_def triv_l_def option_l_def LNew_def
+          split: md_prio.splits md_triv.splits option.splits)
+
+      hence P1sm' : "P1 (snd m')" using M unfolding Sm' by auto
+
+      (* next: step to the end of cond. *)
+
+      have Sub : "|gs| {P2} [G Sif' [body]] @ c'"
+      proof
+        fix mp2 :: "('a, 'b) state"
+
+        assume MP2 : "P2 (snd mp2)"
+
+        assume Cont2 : "s_cont mp2 = [G Sif' [body]] @ c'"
+
+        show "safe gs mp2"
+        proof(cases "get_cond (snd mp2)")
+          case None
+
+          show ?thesis sorry (* rule out this case with valid-sets constraints on predicates *)
+        next
+          case Some' : (Some cnd)
+          then show ?thesis 
+          proof(cases "sem_step gs mp2")
+            case None'' : None
+
+            then have False using Cont2 H0
+              by(auto simp add: sem_step_def)
+
+            then show ?thesis by auto
+
+          next
+            case Some'' : (Some mp2')
+
+            have F_eq' : "sem_step \<lparr> s_sem = f \<rparr> mp2 = Some mp2'"
+              using sym[OF dominant_pcomps'[OF Hpres Hnemp Hdom]] Cont2 Some'' H0
+              by(simp add: sem_step_def)
+
+            (* this will need to be shown using valid-sets. *)
+            have MP2'_valid : "\<And> p . fst (snd (snd mp2)) \<noteq> mdp p None" sorry
+
+            have Mp2'_p2 : "P2 (snd mp2')"
+              using Cont2 Hsyn H0 MP2 F_eq' MP2'_valid Some' unfolding HF
+              by(cases mp2; cases mp2'; 
+                  auto simp add: s_cont_def sem_step_def imp_sem_l_gen_def imp_ctl_sem_def imp_sem_lifting_gen_def
+                  schem_lift_defs 
+                  merge_l_def fst_l_def snd_l_def prio_l_def triv_l_def option_l_def LNew_def
+                  get_cond_def
+                  split: md_prio.splits md_triv.splits option.splits)
+
+
+            show ?thesis
+            proof(cases cnd)
+              case True
+        
+              have Mp2'_cond : "get_cond (snd mp2') = Some True" 
+                using Cont2 Hsyn H0 MP2 F_eq' MP2'_valid True Some' unfolding HF
+                by(cases mp2; cases mp2'; 
+                    auto simp add: s_cont_def sem_step_def imp_sem_l_gen_def imp_ctl_sem_def imp_sem_lifting_gen_def
+                    schem_lift_defs 
+                    merge_l_def fst_l_def snd_l_def prio_l_def triv_l_def option_l_def LNew_def
+                    get_cond_def
+                    split: md_prio.splits md_triv.splits option.splits)
+
+              have Mp2'_p2_true :  "P2 (snd mp2') \<and> get_cond (snd mp2') = Some True"
+                using Mp2'_p2 Mp2'_cond
+                by auto
+
+              have Mp2'_cont : "s_cont mp2' = [body] @ c'"
+                using Cont2 Hsyn H0 MP2 F_eq' MP2'_valid True Some' unfolding HF
+                by(cases mp2; cases mp2'; 
+                    auto simp add: s_cont_def sem_step_def imp_sem_l_gen_def imp_ctl_sem_def imp_sem_lifting_gen_def
+                    schem_lift_defs 
+                    merge_l_def fst_l_def snd_l_def prio_l_def triv_l_def option_l_def LNew_def
+                    get_cond_def
+                    split: md_prio.splits md_triv.splits option.splits)
+
+              have Mp2'_safe : "safe gs mp2'"
+                using guardedD[OF Gtrue Mp2'_p2_true Mp2'_cont] by auto
+
+              show ?thesis
+              proof
+                fix mz
+                assume Exec : "sem_exec_p gs mp2 mz"
+
+                show "imm_safe gs mz" using Exec unfolding sem_exec_p_def
+                proof(cases rule: rtranclp.cases)
+                  case rtrancl_refl
+
+                  then have "(\<exists>m'. sem_step gs mz = Some m')"
+                    using Some'' unfolding imm_safe_def sem_step_p_eq
+                    by(cases mp2'; auto)
+
+                  then show ?thesis unfolding imm_safe_def sem_step_p_eq by auto
+                next
+                  case (rtrancl_into_rtrancl b)
+
+                  have Step : "sem_step_p gs mp2 mp2'" using Some''
+                    unfolding sem_step_p_eq
+                    by auto
+        
+                  have Exec_final : "sem_exec_p gs mp2' mz"
+                    using rtranclp_bisect1
+                      [OF sem_step_determ rtrancl_into_rtrancl(1)
+                          Step rtrancl_into_rtrancl(2)]
+                    unfolding sem_exec_p_def
+                    by auto
+        
+                  show ?thesis using safeD[OF Mp2'_safe Exec_final] by auto 
+                qed
+              qed
+
+            next
+              case False
+
+              have Mp2'_cond : "get_cond (snd mp2') = Some False" 
+                using Cont2 Hsyn H0 MP2 F_eq' MP2'_valid False Some' unfolding HF
+                by(cases mp2; cases mp2'; 
+                    auto simp add: s_cont_def sem_step_def imp_sem_l_gen_def imp_ctl_sem_def imp_sem_lifting_gen_def
+                    schem_lift_defs 
+                    merge_l_def fst_l_def snd_l_def prio_l_def triv_l_def option_l_def LNew_def
+                    get_cond_def
+                    split: md_prio.splits md_triv.splits option.splits)
+
+              have Mp2'_p2_false :  "P2 (snd mp2') \<and> get_cond (snd mp2') = Some False"
+                using Mp2'_p2 Mp2'_cond
+                by auto
+
+              have Mp2'_cont : "s_cont mp2' = [] @ c'"
+                using Cont2 Hsyn H0 MP2 F_eq' MP2'_valid False Some' unfolding HF
+                by(cases mp2; cases mp2'; 
+                    auto simp add: s_cont_def sem_step_def imp_sem_l_gen_def imp_ctl_sem_def imp_sem_lifting_gen_def
+                    schem_lift_defs 
+                    merge_l_def fst_l_def snd_l_def prio_l_def triv_l_def option_l_def LNew_def
+                    get_cond_def
+                    split: md_prio.splits md_triv.splits option.splits)
+
+              have Mp2'_safe : "safe gs mp2'"
+                using guardedD[OF Gfalse Mp2'_p2_false Mp2'_cont] by auto
+
+              show ?thesis
+              proof
+                fix mz
+                assume Exec : "sem_exec_p gs mp2 mz"
+
+                show "imm_safe gs mz" using Exec unfolding sem_exec_p_def
+                proof(cases rule: rtranclp.cases)
+                  case rtrancl_refl
+
+                  then have "(\<exists>m'. sem_step gs mz = Some m')"
+                    using Some'' unfolding imm_safe_def sem_step_p_eq
+                    by(cases mp2'; auto)
+
+                  then show ?thesis unfolding imm_safe_def sem_step_p_eq by auto
+                next
+                  case (rtrancl_into_rtrancl b)
+
+                  have Step : "sem_step_p gs mp2 mp2'" using Some''
+                    unfolding sem_step_p_eq
+                    by auto
+        
+                  have Exec_final : "sem_exec_p gs mp2' mz"
+                    using rtranclp_bisect1
+                      [OF sem_step_determ rtrancl_into_rtrancl(1)
+                          Step rtrancl_into_rtrancl(2)]
+                    unfolding sem_exec_p_def
+                    by auto
+        
+                  show ?thesis using safeD[OF Mp2'_safe Exec_final] by auto 
+                qed
+              qed
+            qed
+          qed
+        qed
+      qed
+
+      have Guard' : "|gs| {P1} [cond] @ ([G Sif' [body]] @ c')"
+        using HTE[OF Hcond Sub] by auto
+
+      have Safe' : "safe gs m'" using guardedD[OF Guard' P1sm' CM'] by auto
+
+      show "safe gs m"
+      proof
+        fix mz
+
+        assume Z: "sem_exec_p gs m mz"
+
+        then show "imm_safe gs mz" unfolding sem_exec_p_def
+        proof(cases rule: rtranclp.cases)
+          case rtrancl_refl
+
+          then have "(\<exists>m'. sem_step gs mz = Some m')"
+            using Some unfolding imm_safe_def sem_step_p_eq
+            by(cases m'; auto)
+
+          then show ?thesis using Some unfolding imm_safe_def sem_step_p_eq
+            by(auto)
+        next
+          case (rtrancl_into_rtrancl b)
+
+          have Step : "sem_step_p gs m m'" using Some
+            unfolding sem_step_p_eq
+            by auto
+
+          have Exec_final : "sem_exec_p gs m' mz"
+            using rtranclp_bisect1
+              [OF sem_step_determ rtrancl_into_rtrancl(1)
+                  Step rtrancl_into_rtrancl(2)]
+            unfolding sem_exec_p_def
+            by auto
+
+          show ?thesis using safeD[OF Safe' Exec_final] by auto
+        qed
+      qed
+    qed
+  qed
+qed
 
 end
